Hs/Translator/Tests/HsTerm.lean
@@ -20,6 +20,6 @@ namespace Translator.HsTerm.Test
 
     #guard (compile_term Γ (#6 -t> #7 -t> #8) (`#0 `•t `#6 `• (.HsHole (`#5 `•k `#6)))) ==
                   .ok (#0 `@t #6 `@ (#4 `@t #6 `@ (refl! ★ #6)))
-    #eval! DsM.run (compile_term Γ (#6 -t> #7 -t> #8) (`#0 `•t `#6 `• (.HsHole (`#5 `•k `#6))))
+    -- #eval DsM.run (compile_term Γ (#6 -t> #7 -t> #8) (`#0 `•t `#6 `• (.HsHole (`#5 `•k `#6))))
 
 end Translator.HsTerm.Test
